# 习题三

随机过程(苏中根) 第三章 Poisson 过程习题

### 1.
- $$ET(t)=ET_0E(-1)^{N(t)}=0$$

- $$Cov(T(s),T(t))=ET(s)T(t)=ET_0^2E(-1)^{N(s+t)}=\sum\limits_{n=0}^\infty(-1)^n\frac{[\lambda(s+t)]^n}{n!}e^{-\lambda(s+t)}=e^{-2\lambda(s+t)}$$
- 同理易知
  - $$EX(t)=0,Cov(X(u),X(v))=EX(u)X(v)=ET_0^2E\int_0^u(-1)^{N(t)}dt\int_0^v(-1)^{N(t)}dt= E(\int_0^u(-1)^{N(t)}dt)^2 + E\int_0^u(-1)^{N(t)}dtE\int_u^v(-1)^{N(t)}dt=u^2+(uv-u^2)e^{-2\lambda t}$$

### 2.
- $$N(t)\sim \mathcal{P}(4t)$$

- $$p(N(0.5)=1)=\frac{4\cdot 0.5}{1!}e^{-4\cdot 0.5}=2e^{-2}$$
- $$p(N(2.5)=5)=\frac{(4\cdot 2.5)^5}{5!}e^{-4\cdot 2.5}=\frac{2500}{3}e^{-10}$$

### 3.
- $$N(t)\sim \mathcal{P}(2t)$$
- $$p(N(1)=2)=\frac{2^2}{2!}e^{-2}=2e^{-2}$$
- $$p(N(1)=2,N(3)=6)=p(N(1)=2,N(3)-N(1)=4)=p(N(1)=2)p(N(2)=4)=2e^{-2}\frac{(4)^4}{4!}e^{-4}=\frac{64}{3}e^{-6}$$
- $$p(N(1)=2|N(3)=6)=\frac{p(N(1)=2,N(3)=6)}{p(N(3)=6)}=\frac{\frac{64}{3}e^{-6}}{\frac{(2\cdot 3)^6}{6!}e^{-6}}=\frac{80}{243}$$
- $$p(N(3)=6|N(1)=2)=\frac{p(N(1)=2,N(3)=6)p(N(3)=6)}{p(N(1)=2)}=\frac{32}{3e^4}$$

### 4.
- $$N(t)\sim \mathcal{P}(2t)$$
- $$p(N(1)\leq 2)=p(N(1)=0)+p(N(1)=1)+p(N(1)=2)=e^{-2}+2e^{-2}+2e^{-2}=5e^{-2}$$
- $$p(N(1)=1,N(2)=3)=p(N(1)=1)p(N(1)=2)=3e^{-2}$$
- $$p(N(1)\geq 2|N(1)\geq 1)=\frac{p(N(1)\geq 2,N(1)\geq 1)}{p(N(1)\geq 1)}=\frac{p(N(1)\geq 2)}{p(N(1)\geq 1)}=\frac{1-p(N(1)=1)-p(N(1)=0)}{1-p(N(1)=0)}=\frac{e^2-3}{e^2-1}$$

### 5.
- $$N(t)\sim \mathcal{P}(2t)$$
- $$EN(2)=4$$
- $$E(N(1))^2=Var(N(1))+(EN(1))^2=2+2^2=6$$
- $$E(N(1)N(2))=E(N(1)(N(2)-N(1)+N(1)))=(EN(1))^2+E(N(1)^2)=4+6=10$$
- $$E(N(1)N(2)N(3))=E(N(1)N(2)(N(3)-N(2)+N(2)))=EN(1)N(2)EN(1)+EN(1)N(2)^2=EN(1)N(2)EN(1)+( EN(1)[N(1)+(N(2)-N(1))]^2 )=EN(1)N(2)EN(1)+EN(1)^3+2EN(1)^2EN(1)+EN(1)EN(1)^2 =78$$
  - 其中$$EN(1)^3=\lambda^3+3\lambda^2+2\lambda|_{\lambda =2}=22$$
  - 这里不能对$N(1)$做变换,因为$N(2),N(2)-N(1)$不独立,但是$N(1),N(2)-N(1)$是独立的

### 6.
- $$N(t)\sim \mathcal{P}(2t),T\sim U(1,2)$$
- $$E(N(T)|T=t)=E(N())=2t,E(N(T)^2|T=t)=4t^2+2t$$
- $$E(N(T))=\int_1^2\frac{1}{2-1}2tdt=3,Var(N(T))=\int_1^24t^2+2tdt=\frac{31}{3}$$

### 7.
- $$N(t)\sim \mathcal{P}(\lambda t)$$
- $$p(T=t)=p(N(t)\leq k)=\sum\limits_{i=0}^k\frac{(\lambda t)^i}{i!}e^{-\lambda t}$$

### 8.
- $$N(t)\sim \mathcal{P}(2t)$$
- $$p(N(3)=0,N(5)\geq 1)=p(N(3)=0)p(N(5)-N(3)\geq 1)=p(N(3)=0)(1-p(N(2)=0))=e^{-6}(1-e^{-4})$$
- $$p(N(3)=0,N(5)=1)=p(N(3)=0)p(N(2)=1)=e^{-6}\frac{4}{1}e^{-4}=4e^{-10}$$

### 9.
- $$N_\alpha(t)\sim\mathcal{P}(\lambda_1 t),N_\beta(t)\sim\mathcal{P}(\lambda_2 t),N_\gamma(t)\sim\mathcal{P}(\lambda_3 t)$$
- $$p(T=t)=p(N_\alpha(t)\geq 1,N_\beta(t)\geq 1,N_\gamma(t)\geq 1)=(1-p(N_\alpha(t)=0))(1-p(N_\beta(t)=0))(1-p(N_\gamma(t)=0))=(1-e^{-\lambda_1 t})(1-e^{-\lambda_2 t})(1-e^{-\lambda_3 t})$$

### 10.
- 教材 p56 页注记3.9
- 直接用密度函数积分或者用结论:$\int_0^t s\times \frac{1}{t^n}\frac{n!}{(k-1)!(n-k)!}s^{k-1}(t-s)^{n-k}|_{n=k=3}ds=\frac{k}{n+1}t|_{n=k=3}=\frac{3}{4}t$

### 11.
- $$E(S_1S_2|N(1)=2)=E(U_{(1)}U_{(2)})=EU_1U_2=\int_0^1\int_0^1xydxdy=\frac{1}{4}$$
- $$E(S_1+\cdots+S_5|N(1)=5)=E(\sum\limits_{i=1}^5U_{(i)})=E(\sum\limits_{i=1}^5U_i)=\sum\limits_{i=1}^5EU_i=\frac{5}{2}$$

### 12.
- $p(x,y,z)=3!,0<x<y<z<1$,其中$x,y,z$表示$S_1,S_2,S_3$的到达时间,做变换$u=x/y,v=(1-x)/(1-y),w=1-y$则$|\frac{\partial{(x,y,z)}}{\partial(u,v,w)}|=w-w^2$,从而$p_{U,V,W}(u,v,w)=3!(w^2-w),p_{U,V}(u,v)=\int_0^13!(w-w^2)dw=1$

### 13.
- $$p(W>w)=p(\min\limits_{n\geq 1}\{S_n+Z_n\}> w)=p(S_1+Z_1>w,\cdots,S_n+Z_n>w)=p(U_1+Z_1>w,\cdots,U_n+Z_n>w)=[1-p(U_1+Z_1\leq w)]^n=[1-p(U_1\leq w-Z_1)]^n=[1-\int_0^wp_{S_1}(w-u)p(u)du]^n=[1-\frac{1}{t}\int_{0}^{w}p(u)du]^n$$

### 14.
- $$E(S_1|N(t)=2)=\frac{1}{3}t$$
- $$E(S_3|N(t)=5)=\frac{1}{2}t$$

### 15.
- $$E(S_l-S_k|N(t)=n)=E(U_{(l)}-U{(k)})=EU_{(l)}-EU_{(k)}=\frac{l}{n+1}t-\frac{k}{n+1}t=\frac{l-k}{n+1}t$$
- $$E(t-S_k|N(t)=n)=t-E(S_k|N(t)=n)=t-\frac{k}{n+1}t=\frac{n-k+1}{n+1}t$$

### 16.
- $$EZ(t)=E\sum\limits_{k=1}^{N(t)}\xi_ke^{-\gamma(t-S_k)}=\sum\limits_{n=0}^{\infty}E(\sum\limits_{k=1}^n\xi_ke^{-\gamma(t-S_k)})p(N(t)=n)=\sum\limits_{n=0}^{\infty}p(N(t)=n)\sum\limits_{k=1}^nE\xi_kEe^{-\gamma(t-S_k)}$$,其中$$\sum\limits_{k=1}^nE\xi_kEe^{-\gamma(t-S_k)}=\mu E\sum\limits_{k=1}^ne^{-\gamma(t-U_k)}=\frac{\mu n}{\gamma t}(1-e^{-\gamma t})$$,故$$EZ(t)=\frac{\mu}{\gamma t}(1-e^{-\gamma t}) \sum\limits_{n=0}^{\infty}np(N(t)=n) = \frac{\lambda\mu}{\gamma}(1-e^{-\gamma t})$$

- $$EZ(t)^2=E(\sum\limits_{k=1}^{N(t)}\xi_ke^{-\gamma(t-S_k)})^2=\sum\limits_{n=0}^{\infty}E(\sum\limits_{k=1}^n\xi_ke^{-\gamma(t-S_k)})^2p(N(t)=n)= \sum\limits_{n=0}^\infty \{ E\sum\limits_{k=1}^n\xi_k^2e^{-2\gamma(t-S_k)} +E\sum\limits_{i\neq j}\xi_i\xi_je^{-\gamma(2t-S_i-S_j)} \} = \frac{\lambda(\sigma^2+\mu^2)}{2\gamma}(1-e^{-2\gamma t})+\frac{\mu^2\lambda^2}{\gamma^2}(1-e^{-\gamma t})^2$$,故 $$VarZ(t)=EZ(t)^2-(EZ(t))^2=\frac{\lambda(\sigma^2+\mu^2)}{2\gamma}(1-e^{-2\gamma t})$$


[知乎](https://zhuanlan.zhihu.com/p/691693860)
