# 习题二

### 1.
- $$EX_n=E(A\cos\lambda n+B\sin\lambda n)=EAE\cos\lambda n+EBE\sin\lambda n=0$$
- $$Cov(X_n,X_m)=EX_nX_m=E(A\cos\lambda n+B\sin\lambda n)(A\cos\lambda m+B\sin\lambda m)=E( A^2\cos\lambda n\cos\lambda m+B^2\sin\lambda n\sin\lambda m + AB\cos\lambda n\sin\lambda m+AB\sin\lambda n\cos\lambda m )=\cos(\lambda(n-m))$$

### 2.
- $$EZ_n=0,VarZ_n=1\Rightarrow EZ_n^2=1$$
- $$EX_n=E\sum\limits_{i=o}^r\alpha_iZ_{n-i}=\sum\limits_{i=o}^r\alpha_iEZ_{n-i}=0$$
- 
  - 若$|m-n|>r$,则$Cov(X_n,X_m)=E\sum\limits_{some\;i\neq j}\alpha_i\alpha_j Z_{n-i}Z_{n-j}=0$因为$Z_{n-i},Z_{n-j}$独立且$EZ_{n-i}=EZ_{n-j}=0$
  - 若$s=|m-n|\leq r$,则不妨设$m\geq n$,从而有$Cov(X_n,X_m)=E\sum\limits_{i=0}^{r-s+1}\alpha_{r-i}Z_{m-r+i}\alpha_{r-s-i}Z_{n-(r-s)+i}=\sum\limits_{i=0}^{r-s+1}\alpha_{r-i}\alpha_{r-s-i}$

### 3.
- 两侧求均值有$EX_n=\alpha EX_{n-1}+EZ_n\Rightarrow EX_n=0$
- 两侧求方差有$VarX_n=\alpha^2VarX_{n-1} + VarZ_n,\Rightarrow VarX_n=\frac{1}{1-\alpha^2}$,则$m=0$时满足所需证的等式
- 不妨设$m>0,$不然有$Cov(X_n,X_{n+m})=Cov(X_{n+m},X_n)\overset{i=n+m,j=-m>0}{=}Cov(X_i,X_{i+j})$
  - 根据递推关系有 $$X_{n+m}=\alpha^mX_n+\alpha^{m-1}Z_{n+1}+\cdots+Z_{n+m}$$,从而有 $$Cov(X_n,X_{n+m})=EX_nX_{n+m}=E\{ \alpha^mX_n^2+\alpha^{m-1}X_nZ_{n+1}+\cdots +X_nZ_{n+m}\}=\alpha^m EX_n^2=\frac{\alpha^m}{1-\alpha^2}$$.得证

### 4.
- $$X(t)\sim \mathcal{N}(0,\cos^2(\theta t)+\sin^2(\theta t))=\mathcal{N}(0,1),\forall t\in R$$

### 5.
- $$E\xi_i=\frac{1}{2},Var\xi_i=\frac{1}{4},E\xi_i^2=\frac{1}{2}$$
- $$EV_n=\sum\limits_{i=1}^\infty\frac{1}{2^{i+1}}=\frac{1}{2}$$
- $$EV^2_n=E(\sum\limits_{i=1}^\infty\frac{1}{2^i})^2=\lim\limits_{m\to\infty}\{ \sum\limits_{i=1}^m\frac{E\xi_{n+i}^2}{4^i}+\sum\limits_{i=1}^{m-1}\sum\limits_{j=i+1}^m\frac{E\xi_{n+i}E\xi_{n+j}}{2^i2^j}\}=\frac{3}{4}$$
  - $$VarV_n=EV^2_n-(EV_n)^2=\frac{3}{4}-\frac{1}{4}=\frac{1}{2}$$
- 从而$m=0$时,$Cov(V_n,V_{n+m})=VarV_n=\frac{1}{2}$
  -  当$m\neq 0$,不妨取$m>0$(理由类似第三题),此时有
     -  $$EV_nV_{n+m}=E\sum\limits_{i=1}^\infty\frac{\xi_{n+i}}{2^i}\sum\limits_{i=1}^\infty\frac{\xi_{nm+i}}{2^i}=(\sum\limits_{i=1}^m\frac{\xi_{n+i}}{2^i}+\frac{1}{2^m}\sum\limits_{i=1}^\infty\frac{\xi_{n+m+i}}{2^i})\sum\limits_{i=1}^\infty\frac{\xi_{n+m+i}}{2^i}=\frac{1}{2^m}\frac{3}{4}+\frac{1}{4}(1-\frac{1}{2^m})=\frac{1}{2^{m+1}}+\frac{1}{4}$$
     -  故有$Cov(V_n,V_{n+m})=\frac{1}{2^{m+1}}$,对$m=0$也符合
  - 综上$Cov(V_n,V_{n+m})=\frac{1}{2^{m+1}}$
- $$(\xi_{n_1+n},\xi_{n_2+n},\cdots,\xi_{n_s+n})\overset{d}{=}(\xi_{n_1},\xi_{n_2},\cdots,\xi_{n_s})$$

从而

$$(V_{n_1+n},V_{n_2+n},\cdots,V_{n_s+n})\overset{d}{=}(V_{n_1},V_{n_2},\cdots,V_{n_s})$$

### 6.
- $$p(1_{\xi_k\leq t}=1)=t,p(1_{\xi_k\leq t}=0)=1-t$$

- $$EX(t)=E\frac{1}{n}\sum\limits_{k=1}^n1_{\xi_k\leq t}=\frac{1}{n}\sum\limits_{k=1}^nE1_{\xi_k\leq 1}=\frac{1}{n}nt=t \implies EX(t)=t$$

- $Cov(X(s),X(t))=EX(s)X(t)-EX(s)EX(t)$

    - 其中
 
 - $$EX(s)X(t)=E\frac{1}{n^2}\sum\limits_{i=1}^n1_{\xi_i\leq s}\sum\limits_{j=1}^n1_{\xi_j\leq t}=\frac{1}{n}E( \sum\limits_{i=1}^n1_{\xi_i\leq s}1_{\xi_i\leq t} +\sum\limits_{i\neq j}1_{\xi_i\leq s}1_{\xi_j\leq t})=\frac{1}{n^2}( n\min\{s,t\} + (n^2-n)st )= \frac{\min\{s,t\}+(n-1)st}{n}$$
  - $\implies Cov(X(s),X(t))=\frac{\min\{s,t\}+(n-1)st}{n}-st=\frac{\min\{s,t\}-st}{n}$
