### 1 

样本平均: $\mu=E X(t)=E X_0 E(-1)^{N(t)}=0$

时间平均 $X_T=\frac{1}{T} \int_0^T X_0(-1)^{N(t)} d t=0$ (对称)

于是 $\tau = \lim\limits_{T\to\infty} X_T=0$

故 $\tau=\mu$.从而满足均值遍历性。

### 2
$$
\begin{aligned}
& \mu=E X(t)=e^{-\alpha t / 2} E B\left(e^{\alpha t}\right)=0 . \\
& X_T=\frac{1}{T} \int_0^{\top} e^{-\alpha t/2} B\left(e^{\alpha t}\right) d t=0 \implies \tau = 0 \\
& \Rightarrow \tau=\mu .
\end{aligned}
$$

### 3
$$
E X_n=\begin{cases}
0 & n=0 \\
\lambda E x_{n-1} & n \geq 1
\end{cases}
$$

$\Rightarrow \mu=E X_n=0$

$$
X_n=Z_n+\lambda Z_{n-1}+\cdots+\lambda^n Z_0
$$
$r_X(k)=E X_0 X_k=E Z_0\left(Z_n+\cdots+\lambda^k Z_0\right)=\lambda^k E Z_0^2=\frac{\lambda^k \sigma^2}{1-\lambda^2}$

$\lim\limits_{k \rightarrow \infty} r_X(k)=0=\mu^2$

故 $X$ 满足均值遍历性

### 4
显然 $X_n$ 平稳

$\mu_X=E X_n=E\left(\frac{\xi_n+\cdots+\xi_{n-k}}{k+1}\right)=\mu$.

取 $l>2k$ 充分大,则有

$$r_X(k) = E\left(\frac{\xi_k+\cdots+\xi_{0}}{k+1}\right)\left(\frac{\xi_{k+l}+\cdots+\xi_l}{k+1}\right)=E\xi_k E\xi_{k+l}=\mu^2$$

于是

$$\lim\limits_{l\to\infty}r_X(l)=\mu_X^2=\mu^2$$

从而满足均值遍历性

### 5
数分知识. $x_n \to a \implies \frac{1}{n} \sum\limits_{i=1}^n x_i \to a$.

$X$ 满足均值遍历性 $\implies r_x(k) \rightarrow \mu^2 \implies \frac{1}{n} \sum\limits_{k=1}^n r_x(k)=\mu^2$


反过来,因为 

$\frac{1}{n^2} \sum\limits_{k=1}^n\left(r_{X}({k})-\mu^2\right) \leq \frac{1}{n^2} \sum\limits_{k=1}^{n} k\left(r_X(k)-\mu^2\right) \leq \frac{1}{{n}^2} \sum\limits_{{k}=1}^{{n}} {n}\left(r_{X}({k})-\mu^2\right)$

两边同时取极限得到左右两边均为 0 ,所以 

$$\lim _{{n} \rightarrow \infty} \frac{1}{{n}^2} \sum_{{k}=1}^{{n}} {k}\left(r_{{X}}({k})-\mu^2\right)=0$$

于是

$$\frac{1}{n^2}\sum\limits_{k=1}^n (n-k)(r_X(k)-\mu^2)\to 0$$

从而满足均值遍历性
